Clean up LL(1) correctness proof for readability

LL1/Parser.v
@@ -99,12 +99,10 @@ Definition mkParseTable g fuel :=
       end
   in  fold_right addProd (SymbolMap.empty (SymbolMap.t (list production))) g.
 
-
-Fixpoint mkTree 
-         (tbl : parse_table)
-         (sym : symbol)
-         (input : list string)
-         (fuel : nat) : (option tree * list string) :=
+Fixpoint parse (tbl : parse_table)
+               (sym : symbol)
+               (input : list string)
+               (fuel : nat) : (option tree * list string) :=
   match fuel with
   | O => (None, input)
   | S n => 
@@ -119,7 +117,7 @@ Fixpoint mkTree
       match parseTableLookup sym (T token) tbl with
       | None => (None, input)
       | Some gamma =>
-        match mkForest tbl gamma input n with
+        match parseForest tbl gamma input n with
         | (None, _) => (None, input)
         | (Some sts, input') =>
           (Some (Node x sts), input')
@@ -127,20 +125,21 @@ Fixpoint mkTree
       end
     end
   end
-with mkForest (tbl : parse_table) 
-              (gamma : list symbol)
-              (input : list string)
-              (fuel : nat) : (option forest * list string) :=
+with parseForest (tbl : parse_table) 
+                 (gamma : list symbol)
+                 (input : list string)
+                 (fuel : nat) :
+                 (option forest * list string) :=
        match fuel with
        | O => (None, input)
        | S n =>
          match gamma with
          | nil => (Some Fnil, input)
          | sym :: gamma' =>
-           match mkTree tbl sym input n with
+           match parse tbl sym input n with
            | (None, _) => (None, input)
            | (Some lSib, input') =>
-             match mkForest tbl gamma' input' n with
+             match parseForest tbl gamma' input' n with
              | (None, _) => (None, input)
              | (Some rSibs, input'') =>
                (Some (Fcons lSib rSibs), input'')
