LL1/ParserTests.v
@@ -4,7 +4,7 @@ Import ListNotations.
 Open Scope string_scope.
 
 Example test1 :
-  mkTree g311ParseTable (NT "S") g311Sentence1 100 =
+  parse g311ParseTable (NT "S") g311Sentence1 100 =
   (Some g311ParseTree1, nil).
 Proof. simpl. reflexivity. Defined.
 
